[IsaSAT] finish backtracking

Weidenbach_Book/IsaSAT/IsaSAT_Backtrack.thy
@@ -739,7 +739,8 @@ definition propagate_bt_wl_D_heur
       ASSERT(cons_trail_Propagated_tr_pre ((-L, i), M));
       M \<leftarrow> cons_trail_Propagated_tr (- L) i M;
       vm \<leftarrow> isa_vmtf_flush_int M vm;
-        heur \<leftarrow> mop_save_phase_heur (atm_of L') (is_neg L') heur;
+      heur \<leftarrow> mop_save_phase_heur (atm_of L') (is_neg L') heur;
+      let S = set_watched_wl_heur W S;
       let S = set_learned_count_wl_heur (clss_size_incr_lcount lcount) S;
       let S = set_aivdom_wl_heur (add_learned_clause_aivdom i vdom) S;
       let S = set_heur_wl_heur (heuristic_reluctant_tick (update_propagation_heuristics glue heur)) S;
@@ -781,7 +782,7 @@ definition propagate_unit_bt_wl_D_int
       let stats = incr_units_since_last_GC (incr_uset stats);
       let S = set_stats_wl_heur stats S;
       let S = set_trail_wl_heur M S;
-      let vm = set_vmtf_wl_heur vm S;
+      let S = set_vmtf_wl_heur vm S;
       let S = set_lbd_wl_heur lbd S;
       let S = set_literals_to_update_wl_heur j S;
       let S = set_heur_wl_heur (heuristic_reluctant_tick (update_propagation_heuristics glue heur)) S;
@@ -1015,11 +1016,7 @@ proof -
     let ?aivdom = \<open>isasat_int.get_aivdom S'\<close>
     let ?b = \<open>fst ?bD'\<close>
     let ?D' = \<open>snd ?bD'\<close>
-    
-    (* obtain M' W' vm clvls cach lbd outl stats heur vdom lcount D' arena b Q' opts old_arena where
-     *   S': \<open>S' = (M', arena, (b, D'), Q', W', vm, clvls, cach, lbd, outl, stats, heur, vdom,
-     *     lcount, opts, old_arena)\<close>
-     *   using S'_S by (cases S') (fastforce simp: twl_st_heur_conflict_ana_def S) *)
+
     let ?vdom = \<open>set (get_vdom_aivdom ?aivdom)\<close>
     have
       M'_M: \<open>(?M', M) \<in> trail_pol (all_atms_st S)\<close>  and
@@ -1351,16 +1348,10 @@ proof -
           by (auto simp: conc_fun_RES RETURN_def)
         done
     qed
-
-(*
-(set_lbd_wl_heur lbd_
-    (set_ccach_max_wl_heur (empty_cach_ref x1a_)
-      (set_vmtf_wl_heur vm_ (set_conflict_wl_heur a_ (set_outl_wl_heur (take 1 x2a_) (set_trail_wl_heur (get_trail_wl_heur S') S'))))),
-   ba_, aa_)
-*)
-    have final: \<open>((set_ccach_max_wl_heur (empty_cach_ref x1a) (set_outl_wl_heur (take 1 x2a) (set_conflict_wl_heur x1b S')), x2c, x1c),
+ 
+    have final: \<open>((set_lbd_wl_heur lbd (set_ccach_max_wl_heur (empty_cach_ref x1a) (set_vmtf_wl_heur vm' (set_conflict_wl_heur x1b (set_outl_wl_heur (take 1 x2a) S')))), x2c, x1c),
           (M, N, Da, NE, UE, NEk, UEk, NS, US, N0, U0, Q, W))
-          \<in> ?shorter\<close>
+          \<in> ?shorter\<close>  (is \<open>((?updated_state, _, _), _) \<in> _\<close>)
       if
         \<open>M \<noteq> []\<close> and
         \<open>- lit_of (hd M) \<in># \<L>\<^sub>a\<^sub>l\<^sub>l (all_atms_st S)\<close> and
@@ -1377,7 +1368,6 @@ proof -
         vm': \<open>(vm', uu) \<in> {(c, uu). c \<in> isa_vmtf (all_atms_st S) M}\<close>
       for x E' x1 x2 x1a x2a xa Da x1b x2b x1c x2c vm' uu lbd
     proof -
-      term xa
       have x1b_None: \<open>(x1b, None) \<in> option_lookup_clause_rel (all_atms_st S)\<close>
         using that apply (auto simp: S simp flip: all_atms_def)
         done
@@ -1435,8 +1425,7 @@ proof -
       then have max_lvl_le:
         \<open>get_maximum_level M (remove1_mset (- lit_of (hd M)) (the Da)) < count_decided M\<close>
         using get_maximum_level_mono[OF Da_D', of M] by auto
-      have \<open>(set_ccach_max_wl_heur (empty_cach_ref x1a) (set_outl_wl_heur (take 1 x2a) (set_conflict_wl_heur x1b S')),
-        del_conflict_wl (M, N, Da, NE, UE, NEk, UEk, NS, US, N0, U0, Q, W))
+      have \<open>(?updated_state, del_conflict_wl (M, N, Da, NE, UE, NEk, UEk, NS, US, N0, U0, Q, W))
         \<in> twl_st_heur_bt\<close>
         using S'_S x1b_None cach out vm' cach unfolding twl_st_heur_bt_def st
         by (auto simp: twl_st_heur_def del_conflict_wl_def S twl_st_heur_bt_def
@@ -1581,7 +1570,7 @@ proof -
     show ?thesis
       supply [[goals_limit=1]]
       unfolding extract_shorter_conflict_list_heur_st_def
-        empty_conflict_and_extract_clause_def S prod.simps hd_M'_M
+        empty_conflict_and_extract_clause_def S prod.simps
       apply (rewrite at  \<open>let _ = list_update _ _ _ in _ \<close>Let_def)
       apply (rewrite at  \<open>let _ =  get_trail_wl_heur S' in _ \<close>Let_def)
       apply (rewrite at  \<open>let _ =  get_clauses_wl_heur S' in _ \<close>Let_def)
@@ -1591,6 +1580,7 @@ proof -
       apply (rewrite at  \<open>let _ =  get_conflict_wl_heur S' in _ \<close>Let_def)
       apply (rewrite at  \<open>let _ =  get_conflict_cach S' in _ \<close>Let_def)
       apply (rewrite at  \<open>let _ = empty_cach_ref _ in _ \<close> Let_def)
+      unfolding hd_M'_M
       apply (subst case_prod_beta)
       apply (subst extract_shorter_conflict_wl_alt_def)
       apply (refine_vcg isa_minimize_and_extract_highest_lookup_conflict[THEN order_trans]
@@ -1604,13 +1594,10 @@ proof -
       subgoal using trail_nempty using M'_M by (auto simp: trail_pol_def ann_lits_split_reasons_def)
       subgoal using \<open>0 < length ?outl\<close> .
       subgoal unfolding hd_M'_M[symmetric] by (rule lookup_conflict_remove1_pre)
-        apply (rule vmtf_mark_to_rescore_also_reasons[unfolded hd_M'_M[symmetric]]; assumption?)
+        apply (rule vmtf_mark_to_rescore_also_reasons; assumption?)
       subgoal using trail_nempty .
       subgoal using pre2  by (auto simp: S all_atms_def)
-      subgoal using uM_\<L>\<^sub>a\<^sub>l\<^sub>l[unfolded hd_M'_M[symmetric]] by (auto simp: S all_atms_def)
-      apply (subst hd_M'_M[symmetric])+
-      apply (rule isa_minimize_and_extract_highest_lookup_conflict[unfolded hd_M'_M[symmetric], THEN order_trans])
-      apply (rule GG[unfolded hd_M'_M[symmetric]])
+      subgoal using uM_\<L>\<^sub>a\<^sub>l\<^sub>l by (auto simp: S all_atms_def)
       subgoal premises p
         using bounded p by (auto simp: S empty_cach_ref_pre_def cach_refinement_alt_def
           intro!: IsaSAT_Lookup_Conflict.bounded_included_le simp: all_atms_def simp del: isasat_input_bounded_def
@@ -1621,17 +1608,16 @@ proof -
             simp del: isasat_input_bounded_def)
       subgoal using trail_nempty by fast
       subgoal using uM_\<L>\<^sub>a\<^sub>l\<^sub>l .
-      subgoal unfolding hd_M'_M[symmetric] by assumption+
-      apply (unfold hd_M'_M[symmetric], assumption)+
+      apply (assumption)+
       subgoal
         using trail_nempty uM_\<L>\<^sub>a\<^sub>l\<^sub>l
         unfolding S[symmetric]
-        by (auto dest!: final simp: clss0)
-         apply assumption+
-      subgoal
+        by (auto dest!: simp: clss0)
+      apply assumption+
+      subgoal for lbd uu vm uua x E' x1 x2 x1a x2a xa Da a b aa ba
         using trail_nempty uM_\<L>\<^sub>a\<^sub>l\<^sub>l apply -
-        unfolding S[symmetric] all_lits_alt_def[symmetric] hd_M'_M[symmetric]
-        apply (rule final[unfolded hd_M'_M[symmetric] clss0 Multiset.empty_neutral])
+        unfolding S[symmetric] all_lits_alt_def[symmetric]
+        by (rule final[unfolded clss0 Multiset.empty_neutral])
       done
   qed
 
@@ -1658,21 +1644,34 @@ proof -
     obtain M N D NE UE NEk UEk NS US N0 U0 Q W where
       T': \<open>T' = (M, N, D, NE, UE, NEk, UEk, NS, US, N0, U0, Q, W)\<close>
       by (cases T')
-    obtain M' W' vm clvls cach lbd outl stats arena D' Q' heur vdom lcount opts old_arena where
-      T: \<open>T = (M', arena, D', Q', W', vm, clvls, cach, lbd, outl, stats, heur, vdom, lcount,
-         opts, old_arena)\<close>
-      using TT' by (cases T) (auto simp: twl_st_heur_bt_def T' del_conflict_wl_def)
+
+    let ?M' = \<open>get_trail_wl_heur T\<close>
+    let ?arena = \<open>get_clauses_wl_heur T\<close>
+    let ?D' = \<open>get_conflict_wl_heur T\<close>
+    let ?W' = \<open>get_watched_wl_heur T\<close>
+    let ?vm = \<open>get_vmtf_heur T\<close>
+    let ?clvls = \<open>get_count_max_lvls_heur T\<close>
+    let ?cach = \<open>get_conflict_cach T\<close>
+    let ?outl = \<open>get_outlearned_heur T\<close>
+    let ?lcount = \<open>get_learned_count T\<close>
+    let ?aivdom = \<open>isasat_int.get_aivdom T\<close>
+
+    let ?vdom = \<open>set (get_vdom_aivdom ?aivdom)\<close>
+    (* obtain M' W' vm clvls cach lbd outl stats arena D' Q' heur vdom lcount opts old_arena where
+     *   T: \<open>T = (M', arena, D', Q', W', vm, clvls, cach, lbd, outl, stats, heur, vdom, lcount,
+     *      opts, old_arena)\<close>
+     *   using TT' by (cases T) (auto simp: twl_st_heur_bt_def T' del_conflict_wl_def) *)
     have
-      vm: \<open>vm \<in> isa_vmtf (all_atms_st T') M\<close> and
-      M'M: \<open>(M', M) \<in> trail_pol (all_atms_st T')\<close> and
+      vm: \<open>?vm \<in> isa_vmtf (all_atms_st T') M\<close> and
+      M'M: \<open>(?M', M) \<in> trail_pol (all_atms_st T')\<close> and
       lits_trail: \<open>literals_are_in_\<L>\<^sub>i\<^sub>n_trail (all_atms_st T') (get_trail_wl T')\<close>
       using TT' by (auto simp: twl_st_heur_bt_def del_conflict_wl_def all_atms_st_def
-          all_atms_def[symmetric] T T' all_lits_st_alt_def[symmetric])
+          all_atms_def[symmetric] T' all_lits_st_alt_def[symmetric])
 
     obtain vm0 where
-      vm: \<open>(vm, vm0) \<in> Id \<times>\<^sub>r distinct_atoms_rel (all_atms_st T')\<close> and
+      vm: \<open>(?vm, vm0) \<in> Id \<times>\<^sub>r distinct_atoms_rel (all_atms_st T')\<close> and
       vm0: \<open>vm0 \<in> vmtf (all_atms_st T') M\<close>
-      using vm unfolding isa_vmtf_def by (cases vm) auto
+      using vm unfolding isa_vmtf_def by (cases ?vm) auto
 
     have [simp]:
        \<open>LK' = lit_of (hd (get_trail_wl T'))\<close>
@@ -1682,19 +1681,19 @@ proof -
     have n: \<open>n = get_maximum_level M (remove1_mset (- lit_of (hd M)) (mset C))\<close> and
       eq: \<open>equality_except_conflict_wl T' S'\<close> and
       \<open>the D = mset C\<close> \<open>D \<noteq> None\<close> and
-      clss_eq: \<open>get_clauses_wl_heur S = arena\<close> and
+      clss_eq: \<open>get_clauses_wl_heur S = ?arena\<close> and
       n: \<open>n < count_decided (get_trail_wl T')\<close> and
       bounded: \<open>isasat_input_bounded (all_atms_st T')\<close> and
       T_T': \<open>(T, del_conflict_wl T') \<in> twl_st_heur_bt\<close> and
       n2: \<open>n = get_maximum_level M (remove1_mset (- lit_of (hd M)) (the D))\<close> and
       lcount: \<open>get_learned_count T = get_learned_count S\<close>
-      using TT' KK' by (auto simp: T T' twl_st_heur_bt_def del_conflict_wl_def all_atms_st_def
-          T T' all_lits_st_alt_def[symmetric] simp flip: all_atms_def
+      using TT' KK' by (auto simp: T' twl_st_heur_bt_def del_conflict_wl_def all_atms_st_def
+          T' all_lits_st_alt_def[symmetric] simp flip: all_atms_def
           simp del: isasat_input_bounded_def)
     have [simp]: \<open>get_trail_wl S' = M\<close>
       using eq \<open>the D = mset C\<close> \<open>D \<noteq> None\<close> by (cases S'; auto simp: T')
-    have [simp]: \<open>get_clauses_wl_heur S = arena\<close>
-      using TT' by (auto simp: T T')
+    have [simp]: \<open>get_clauses_wl_heur S = ?arena\<close>
+      using TT' by (auto simp: T')
 
     have n_d: \<open>no_dup M\<close>
       using M'M unfolding trail_pol_def by auto
@@ -1703,7 +1702,7 @@ proof -
       by (auto simp: out_learned_def)
 
     show ?thesis
-      unfolding T' find_decomp_wl_st_int_def prod.case T
+      unfolding T' find_decomp_wl_st_int_def prod.case Let_def
       apply (rule bind_refine_res)
        prefer 2
        apply (rule order.trans)
@@ -1723,7 +1722,7 @@ proof -
        apply (rule order.refl)
       using T_T' n_d lcount (*TODO Tune proof*)
       apply (cases \<open>get_vmtf_heur T\<close>)
-      apply (auto simp: find_decomp_wl_def twl_st_heur_bt_def T T' del_conflict_wl_def
+      apply (auto simp: find_decomp_wl_def twl_st_heur_bt_def T' del_conflict_wl_def
           dest: no_dup_appendD
           simp flip: all_atms_def n2
           intro!: RETURN_RES_refine
@@ -1881,36 +1880,52 @@ proof -
       using \<open>(TnC, T') \<in> ?shorter S' S\<close> \<open>1 < length C\<close> find_decomp
       apply (cases U')
       by (auto simp: find_lit_of_max_level_wl_def T' intro: literals_are_in_\<L>\<^sub>i\<^sub>n_mono)
-    obtain M1' vm' W' clvls cach lbd outl stats heur vdom lcount arena D'
-        Q' opts
-      where
-        U: \<open>U = (M1', arena, D', Q', W', vm', clvls, cach, lbd, outl, stats, heur,
-           vdom, lcount, opts, [])\<close>
+
+    let ?M1' = \<open>get_trail_wl_heur U\<close>
+    let ?arena = \<open>get_clauses_wl_heur U\<close>
+    let ?D' = \<open>get_conflict_wl_heur U\<close>
+    let ?W' = \<open>get_watched_wl_heur U\<close>
+    let ?vm' = \<open>get_vmtf_heur U\<close>
+    let ?clvls = \<open>get_count_max_lvls_heur U\<close>
+    let ?cach = \<open>get_conflict_cach U\<close>
+    let ?outl = \<open>get_outlearned_heur U\<close>
+    let ?lcount = \<open>get_learned_count U\<close>
+    let ?heur = \<open>get_heur U\<close>
+    let ?lbd = \<open>get_lbd U\<close>
+    let ?aivdom = \<open>isasat_int.get_aivdom U\<close>
+
+    let ?vdom = \<open>set (get_vdom_aivdom ?aivdom)\<close>
+    (* obtain M1' vm' W' clvls cach lbd outl stats heur vdom lcount arena D'
+     *     Q' opts
+     *   where
+     *     U: \<open>U = (M1', arena, D', Q', W', vm', clvls, cach, lbd, outl, stats, heur,
+     *        vdom, lcount, opts, [])\<close>
+     *    *)
+    have old: \<open>get_old_arena U = []\<close>
       using UU' find_decomp by (cases U) (auto simp: U' T' twl_st_heur_bt_def all_atms_def[symmetric])
-    let ?vdom = \<open>set (get_vdom_aivdom vdom)\<close>
     have [simp]:
        \<open>LK' = lit_of (hd M)\<close>
        \<open>LK = LK'\<close>
        using KK' SS' by (auto simp: equality_except_conflict_wl_get_trail_wl S')
     have
-      M1'_M1: \<open>(M1', M1) \<in> trail_pol (all_atms_st U')\<close> and
-      W'W: \<open>(W', W) \<in> \<langle>Id\<rangle>map_fun_rel (D\<^sub>0 (all_atms_st U'))\<close> and
-      vmtf: \<open>vm' \<in> isa_vmtf (all_atms_st U') M1\<close> and
+      M1'_M1: \<open>(?M1', M1) \<in> trail_pol (all_atms_st U')\<close> and
+      W'W: \<open>(?W', W) \<in> \<langle>Id\<rangle>map_fun_rel (D\<^sub>0 (all_atms_st U'))\<close> and
+      vmtf: \<open>?vm' \<in> isa_vmtf (all_atms_st U') M1\<close> and
       n_d_M1: \<open>no_dup M1\<close> and
-      empty_cach: \<open>cach_refinement_empty (all_atms_st U') cach\<close> and
-      \<open>length outl = Suc 0\<close> and
-      outl: \<open>out_learned M1 None outl\<close> and
+      empty_cach: \<open>cach_refinement_empty (all_atms_st U') ?cach\<close> and
+      \<open>length ?outl = Suc 0\<close> and
+      outl: \<open>out_learned M1 None ?outl\<close> and
       vdom: \<open>vdom_m (all_atms_st U') W N \<subseteq> ?vdom\<close> and
-      lcount: \<open>clss_size_corr N NE UE NEk UEk NS US N0 U0 lcount\<close> and
+      lcount: \<open>clss_size_corr N NE UE NEk UEk NS US N0 U0 ?lcount\<close> and
       vdom_m: \<open>vdom_m (all_atms_st U') W N \<subseteq> ?vdom\<close> and
-      D': \<open>(D', None) \<in> option_lookup_clause_rel (all_atms_st U')\<close> and
-      valid: \<open>valid_arena arena N ?vdom\<close> and
-      aivdom: \<open>aivdom_inv_dec vdom (dom_m N)\<close> and
+      D': \<open>(?D', None) \<in> option_lookup_clause_rel (all_atms_st U')\<close> and
+      valid: \<open>valid_arena ?arena N ?vdom\<close> and
+      aivdom: \<open>aivdom_inv_dec ?aivdom (dom_m N)\<close> and
       bounded: \<open>isasat_input_bounded (all_atms_st U')\<close> and
       nempty: \<open>isasat_input_nempty (all_atms_st U')\<close> and
-      dist_vdom: \<open>distinct (get_vdom_aivdom vdom)\<close> and
-      heur: \<open>heuristic_rel (all_atms_st U') heur\<close>
-      using UU' by (auto simp: out_learned_def twl_st_heur_bt_def U U' all_atms_def[symmetric]
+      dist_vdom: \<open>distinct (get_vdom_aivdom ?aivdom)\<close> and
+      heur: \<open>heuristic_rel (all_atms_st U') ?heur\<close>
+      using UU' by (auto simp: out_learned_def twl_st_heur_bt_def U' all_atms_def[symmetric]
         aivdom_inv_dec_alt_def)
     have [simp]: \<open>C ! 1 = L'\<close> \<open>C ! 0 = - lit_of (hd M)\<close> and
       n_d: \<open>no_dup M\<close>
@@ -1935,10 +1950,18 @@ proof -
           simp: intro_spec_iff bind_RES)
       ultimately show ?thesis by auto
     qed
-
+thm propagate_bt_wl_D_heur_def
     have propagate_bt_wl_D_heur_alt_def:
-      \<open>propagate_bt_wl_D_heur = (\<lambda>L C (M, N0, D, Q, W0, vm0, y, cach, lbd, outl, stats, heur,
-           vdom, lcount, opts). do {
+      \<open>propagate_bt_wl_D_heur = (\<lambda>L C S. do {
+          let M = get_trail_wl_heur S;
+          let vdom = isasat_int.get_aivdom S;
+          let N0 = get_clauses_wl_heur S;
+          let W0 = get_watched_wl_heur S;
+          let lcount = get_learned_count S;
+          let heur = get_heur S;
+          let stats = get_stats_heur S;
+          let lbd = get_lbd S;
+          let vm0 = get_vmtf_heur S;
           ASSERT(length (get_vdom_aivdom vdom) \<le> length N0);
           ASSERT(length (get_avdom_aivdom vdom) \<le> length N0);
           ASSERT(nat_of_lit (C!1) < length W0 \<and> nat_of_lit (-L) < length W0);
@@ -1949,18 +1972,14 @@ proof -
           glue \<leftarrow> get_LBD lbd;
           let _ = C;
           let b = False;
-          ASSERT(isasat_fast (M, N0, D, Q, W0, vm0, y, cach, lbd, outl, stats, heur,
-            vdom, lcount, opts) \<longrightarrow> append_and_length_fast_code_pre ((b, C), N0));
-          ASSERT(isasat_fast (M, N0, D, Q, W0, vm0, y, cach, lbd, outl, stats, heur,
-             vdom, lcount, opts) \<longrightarrow> clss_size_lcount lcount < sint64_max);
+          ASSERT(isasat_fast S \<longrightarrow> append_and_length_fast_code_pre ((b, C), N0));
+          ASSERT(isasat_fast S \<longrightarrow> clss_size_lcount lcount < sint64_max);
           (N, i) \<leftarrow> fm_add_new b C N0;
           ASSERT(update_lbd_pre ((i, glue), N));
           let N = update_lbd i glue N;
-          ASSERT(isasat_fast (M, N0, D, Q, W0, vm0, y, cach, lbd, outl, stats, heur,
-            vdom, lcount, opts) \<longrightarrow> length_ll W0 (nat_of_lit (-L)) < sint64_max);
+          ASSERT(isasat_fast S \<longrightarrow> length_ll W0 (nat_of_lit (-L)) < sint64_max);
           let W = W0[nat_of_lit (- L) := W0 ! nat_of_lit (- L) @ [(i, L', length C = 2)]];
-          ASSERT(isasat_fast (M, N0, D, Q, W0, vm0, y, cach, lbd, outl, stats, heur,
-            vdom, lcount, opts) \<longrightarrow> length_ll W (nat_of_lit L') < sint64_max);
+          ASSERT(isasat_fast S \<longrightarrow> length_ll W (nat_of_lit L') < sint64_max);
           let W = W[nat_of_lit L' := W!nat_of_lit L' @ [(i, -L, length C = 2)]];
           lbd \<leftarrow> lbd_empty lbd;
           j \<leftarrow> mop_isa_length_trail M;
@@ -1969,12 +1988,19 @@ proof -
           M \<leftarrow> cons_trail_Propagated_tr (- L) i M;
           vm \<leftarrow> isa_vmtf_flush_int M vm;
           heur \<leftarrow> mop_save_phase_heur (atm_of L') (is_neg L') heur;
-          RETURN (M, N, D, j, W, vm, 0,
-            cach, lbd, outl, add_lbd (of_nat glue) stats, heuristic_reluctant_tick (update_propagation_heuristics glue heur),
-            add_learned_clause_aivdom i vdom, clss_size_incr_lcount lcount, opts)
+         let
+            S = set_watched_wl_heur W S;
+            S = set_learned_count_wl_heur (clss_size_incr_lcount lcount) S;
+            S = set_aivdom_wl_heur (add_learned_clause_aivdom i vdom) S;
+            S = set_heur_wl_heur (heuristic_reluctant_tick (update_propagation_heuristics glue heur)) S;
+            S = set_stats_wl_heur (add_lbd (word_of_nat glue) stats) S; S = set_trail_wl_heur M S;
+            S = set_clauses_wl_heur N S; S = set_literals_to_update_wl_heur j S;
+            S = set_count_max_wl_heur 0 S; S = set_vmtf_wl_heur vm S;
+            S = set_lbd_wl_heur lbd S in
+          RETURN S
       })\<close>
       unfolding propagate_bt_wl_D_heur_def Let_def
-      by auto
+      by (auto intro!: ext bind_cong[OF refl])
     have find_new_alt: \<open>SPEC
                  (\<lambda>(N', i). N' = fmupd i (D'', False) N \<and> 0 < i \<and>
                       i \<notin># dom_m N \<and>
@@ -2016,7 +2042,7 @@ proof -
                   L' := W L' @ [(i, - LK', length D'' = 2)]))
           }\<close>
       unfolding propagate_bt_wl_def Let_def find_new_alt nres_monad3
-        U U' H get_fresh_index_wl_def prod.case
+        U' H get_fresh_index_wl_def prod.case
         propagate_bt_wl_def Let_def rescore_clause_def
       by (auto simp: U' RES_RES2_RETURN_RES RES_RETURN_RES uminus_\<A>\<^sub>i\<^sub>n_iff
           uncurry_def RES_RES_RETURN_RES length_list_ge2 C_1_neq_hd
@@ -2030,11 +2056,11 @@ proof -
       by (auto intro!: RES_refine simp: RETURN_def)
 
     obtain vm0 where
-      vm: \<open>(vm', vm0) \<in> Id \<times>\<^sub>r distinct_atoms_rel (all_atms_st U')\<close> and
+      vm: \<open>(?vm', vm0) \<in> Id \<times>\<^sub>r distinct_atoms_rel (all_atms_st U')\<close> and
       vm0: \<open>vm0 \<in> vmtf (all_atms_st U') M1\<close>
-      using vmtf unfolding isa_vmtf_def by (cases vm') auto
+      using vmtf unfolding isa_vmtf_def by (cases ?vm') auto
     have [refine0]:
-      \<open>isa_vmtf_rescore C M1' vm' \<le> SPEC (\<lambda>c. (c, ()) \<in> {((vm), _).
+      \<open>isa_vmtf_rescore C ?M1' ?vm' \<le> SPEC (\<lambda>c. (c, ()) \<in> {((vm), _).
          vm \<in> isa_vmtf (all_atms_st U') M1})\<close>
       apply (rule order.trans)
        apply (rule isa_vmtf_rescore[of \<open>all_atms_st U'\<close>, THEN fref_to_Down_curry2, of _ _ _ C M1 vm0])
@@ -2058,7 +2084,7 @@ proof -
          no_dup M0''}\<close>
       for vm i L Ma M2
     proof -
-      let ?M1' = \<open>cons_trail_Propagated_tr L i M1'\<close>
+      let ?M1' = \<open>cons_trail_Propagated_tr L i ?M1'\<close>
       let ?M1 = \<open>Propagated (-L) i # M1\<close>
 
       have M1'_M1: \<open>(Ma, M2) \<in> trail_pol (all_atms_st U')\<close>
@@ -2083,10 +2109,10 @@ proof -
       	done
     qed
 
-    have [refine0]: \<open>(mop_isa_length_trail M1') \<le> \<Down> {(j, _). j = length M1} (RETURN ())\<close>
+    have [refine0]: \<open>(mop_isa_length_trail ?M1') \<le> \<Down> {(j, _). j = length M1} (RETURN ())\<close>
       by (rule order_trans[OF mop_isa_length_trail_length_u[THEN fref_to_Down_Id_keep, OF _ M1'_M1]])
          (auto simp: conc_fun_RES RETURN_def)
-    have [refine0]: \<open>get_LBD lbd \<le> \<Down> {(_, _). True}(RETURN ())\<close>
+    have [refine0]: \<open>get_LBD ?lbd \<le> \<Down> {(_, _). True}(RETURN ())\<close>
       unfolding get_LBD_def by (auto intro!: RES_refine simp: RETURN_def)
     have [refine0]: \<open>RETURN C
        \<le> \<Down> Id
@@ -2096,9 +2122,9 @@ proof -
       by (auto simp: list_of_mset2_def S')
     have [simp]: \<open>0 < header_size D''\<close> for D''
       by (auto simp: header_size_def)
-    have [simp]: \<open>length arena + header_size D'' \<notin> ?vdom\<close>
-      \<open>length arena + header_size D'' \<notin> vdom_m (all_atms_st U') W N\<close>
-      \<open>length arena + header_size D'' \<notin># dom_m N\<close> for D''
+    have [simp]: \<open>length ?arena + header_size D'' \<notin> ?vdom\<close>
+      \<open>length ?arena + header_size D'' \<notin> vdom_m (all_atms_st U') W N\<close>
+      \<open>length ?arena + header_size D'' \<notin># dom_m N\<close> for D''
       using valid_arena_in_vdom_le_arena(1)[OF valid] vdom
       by (auto 5 1 simp: vdom_m_def)
     have add_new_alt_def: \<open>(SPEC
@@ -2116,9 +2142,9 @@ proof -
       using lits
       by (auto simp: T' vdom_m_def literals_are_\<L>\<^sub>i\<^sub>n_def is_\<L>\<^sub>a\<^sub>l\<^sub>l_def U' all_atms_def
         all_lits_st_def all_lits_def ac_simps)
-    have [refine0]: \<open>fm_add_new False C arena
+    have [refine0]: \<open>fm_add_new False C ?arena
        \<le> \<Down> {((arena', i), (N', i')). valid_arena arena' N' (insert i ?vdom) \<and> i = i' \<and>
-             i \<notin># dom_m N \<and> i \<notin> ?vdom \<and> length arena' = length arena + header_size D'' + length D''}
+             i \<notin># dom_m N \<and> i \<notin> ?vdom \<and> length arena' = length ?arena + header_size D'' + length D''}
           (SPEC
             (\<lambda>(N', i).
                 N' = fmupd i (D'', False) N \<and>
@@ -2133,7 +2159,7 @@ proof -
       using that valid le_C vdom
       by (auto simp: intro!: RETURN_RES_refine valid_arena_append_clause)
     have [refine0]:
-      \<open>lbd_empty lbd \<le> SPEC (\<lambda>c. (c, ()) \<in> {(c, _). c = replicate (length lbd) False})\<close>
+      \<open>lbd_empty ?lbd \<le> SPEC (\<lambda>c. (c, ()) \<in> {(c, _). c = replicate (length ?lbd) False})\<close>
       by (auto simp: lbd_empty_def)
 
     have \<open>literals_are_in_\<L>\<^sub>i\<^sub>n (all_atms_st S') (mset C)\<close>
@@ -2141,9 +2167,9 @@ proof -
     then have C_Suc1_in: \<open>C ! Suc 0 \<in># \<L>\<^sub>a\<^sub>l\<^sub>l (all_atms_st S')\<close>
       using \<open>1 < length C\<close>
       by (cases C; cases \<open>tl C\<close>) (auto simp: literals_are_in_\<L>\<^sub>i\<^sub>n_add_mset)
-    then have \<open>nat_of_lit (C ! Suc 0) < length W'\<close> \<open>nat_of_lit (- lit_of (hd (get_trail_wl S'))) < length W'\<close> and
-     W'_eq:  \<open>W' ! (nat_of_lit (C ! Suc 0)) = W (C! Suc 0)\<close>
-        \<open>W' ! (nat_of_lit (- lit_of (hd (get_trail_wl S')))) = W (- lit_of (hd (get_trail_wl S')))\<close>
+    then have \<open>nat_of_lit (C ! Suc 0) < length ?W'\<close> \<open>nat_of_lit (- lit_of (hd (get_trail_wl S'))) < length ?W'\<close> and
+     W'_eq:  \<open>?W' ! (nat_of_lit (C ! Suc 0)) = W (C! Suc 0)\<close>
+        \<open>?W' ! (nat_of_lit (- lit_of (hd (get_trail_wl S')))) = W (- lit_of (hd (get_trail_wl S')))\<close>
       using uM_\<L>\<^sub>a\<^sub>l\<^sub>l W'W unfolding map_fun_rel_def by (auto simp: image_image S' U' all_atms_st_def)
     have le_C_ge: \<open>length C \<le> uint32_max div 2 + 1\<close>
       using clss_size_uint32_max[OF bounded, of \<open>mset C\<close>] \<open>literals_are_in_\<L>\<^sub>i\<^sub>n (all_atms_st S') (mset C)\<close> list_confl_S'
@@ -2236,7 +2262,7 @@ proof -
         by (auto simp: vdom_m_simps5 vdom_m_def ac_simps)
     qed
 
-    have [refine0]: \<open>mop_save_phase_heur (atm_of (C ! 1)) (is_neg (C ! 1)) heur
+    have [refine0]: \<open>mop_save_phase_heur (atm_of (C ! 1)) (is_neg (C ! 1)) ?heur
     \<le> SPEC
        (\<lambda>c. (c, ())
             \<in> {(c, _). heuristic_rel (all_atms_st U') c})\<close>
@@ -2246,10 +2272,10 @@ proof -
       by (auto intro!: ASSERT_leI save_phase_heur_preI simp: U' S' all_atms_st_def)
     have stuff: \<open>?NUE_before = ?NUE_after\<close>
       by auto
-    have arena_le: \<open>length arena + header_size C + length C \<le> MAX_HEADER_SIZE+1 + r + uint32_max div 2\<close>
-      using r r' le_C_ge by (auto simp: uint32_max_def header_size_def S' U)
-    have avdom: \<open>mset (get_avdom_aivdom vdom) \<subseteq># mset (get_vdom_aivdom vdom)\<close> and
-      ivdom: \<open>mset (get_ivdom_aivdom vdom) \<subseteq># mset (get_vdom_aivdom vdom)\<close>
+    have arena_le: \<open>length ?arena + header_size C + length C \<le> MAX_HEADER_SIZE+1 + r + uint32_max div 2\<close>
+      using r r' le_C_ge by (auto simp: uint32_max_def header_size_def S')
+    have avdom: \<open>mset (get_avdom_aivdom ?aivdom) \<subseteq># mset (get_vdom_aivdom ?aivdom)\<close> and
+      ivdom: \<open>mset (get_ivdom_aivdom ?aivdom) \<subseteq># mset (get_vdom_aivdom ?aivdom)\<close>
       using aivdom unfolding aivdom_inv_dec_alt_def by auto
     have vm: \<open>vm \<in> isa_vmtf (all_atms N (NE + UE)) M1 \<Longrightarrow>
        vm \<in> isa_vmtf (all_atms N (NE + UE)) (Propagated (- lit_of (hd M)) x2a # M1)\<close> for x2a vm
@@ -2260,18 +2286,28 @@ proof -
       using empty_cach n_d_M1 C_L' W'W outl vmtf undef \<open>1 < length C\<close> lits
         uM_\<L>\<^sub>a\<^sub>l\<^sub>l vdom lcount vdom_m dist_vdom heur
       apply (subst propagate_bt_wl_D_alt_def)
-      unfolding U U' H get_fresh_index_wl_def prod.case
+      unfolding U' H get_fresh_index_wl_def prod.case
         propagate_bt_wl_D_heur_alt_def rescore_clause_def
       apply (rewrite in \<open>let _ = _!1 in _\<close> Let_def)
       apply (rewrite in \<open>let _ = update_lbd _ _ _ in _\<close> Let_def)
       apply (rewrite in \<open>let _ = list_update _ (nat_of_lit _) _ in _\<close> Let_def)
       apply (rewrite in \<open>let _ = list_update _ (nat_of_lit _) _ in _\<close> Let_def)
       apply (rewrite in \<open>let _ = False in _\<close> Let_def)
+      apply (rewrite at  \<open>let _ =  get_trail_wl_heur _ in _ \<close>Let_def)
+      apply (rewrite at  \<open>let _ =  get_clauses_wl_heur _ in _ \<close>Let_def)
+      apply (rewrite at  \<open>let _ =  get_vmtf_heur _ in _ \<close>Let_def)
+      apply (rewrite at  \<open>let _ =  get_lbd _ in _ \<close>Let_def)
+      apply (rewrite at  \<open>let _ =  get_aivdom _ in _ \<close>Let_def)
+      apply (rewrite at  \<open>let _ =  get_watched_wl_heur _ in _ \<close>Let_def)
+      apply (rewrite at  \<open>let _ = get_learned_count _ in _ \<close> Let_def)
+      apply (rewrite at  \<open>let _ = get_heur _ in _ \<close> Let_def)
+      apply (rewrite at  \<open>let _ = get_stats_heur _ in _ \<close> Let_def)
+
       apply (refine_rcg cons_trail_Propagated_tr2[of _ _ _ _ _ _ \<open>all_atms_st U'\<close>])
       subgoal using valid by (auto dest!: valid_arena_vdom_subset)
       subgoal  using valid size_mset_mono[OF avdom] by (auto dest!: valid_arena_vdom_subset)
-      subgoal using \<open>nat_of_lit (C ! Suc 0) < length W'\<close> by simp
-      subgoal using \<open>nat_of_lit (- lit_of (hd (get_trail_wl S'))) < length W'\<close>
+      subgoal using \<open>nat_of_lit (C ! Suc 0) < length ?W'\<close> by simp
+      subgoal using \<open>nat_of_lit (- lit_of (hd (get_trail_wl S'))) < length ?W'\<close>
         by (simp add: S' lit_of_hd_trail_def)
       subgoal using le_C_ge .
       subgoal by (auto simp: append_and_length_fast_code_pre_def isasat_fast_def
@@ -2285,9 +2321,9 @@ proof -
       subgoal for x uu x1 x2 vm uua_ glue uub D'' xa x'
         by (auto simp: update_lbd_pre_def arena_is_valid_clause_idx_def)
       subgoal using length_watched_le[of S' S \<open>-lit_of_hd_trail M\<close>] corr SS' uM_\<L>\<^sub>a\<^sub>l\<^sub>l W'_eq S_arena
-         by (auto simp: isasat_fast_def length_ll_def S' U lit_of_hd_trail_def simp flip: all_atms_def)
+         by (auto simp: isasat_fast_def length_ll_def S' lit_of_hd_trail_def simp flip: all_atms_def)
       subgoal using length_watched_le[of S' S \<open>C ! Suc 0\<close>] corr SS' W'_eq S_arena C_1_neq_hd C_Suc1_in
-         by (auto simp: length_ll_def S' U lit_of_hd_trail_def isasat_fast_def simp flip: all_atms_def)
+         by (auto simp: length_ll_def S' lit_of_hd_trail_def isasat_fast_def simp flip: all_atms_def)
       subgoal using D' C_1_neq_hd vmtf avdom
         by (auto simp: DECISION_REASON_def
             dest: valid_arena_one_notin_vdomD
@@ -2311,18 +2347,18 @@ proof -
         unfolding twl_st_heur_def
         using D' C_1_neq_hd vmtf avdom aivdom M1'_M1 bounded nempty r r' arena_le
           set_mset_mono[OF ivdom]
-        by (clarsimp simp add: propagate_bt_wl_D_heur_def twl_st_heur_def
-            Let_def T' U' U rescore_clause_def S' map_fun_rel_def
+        by (clarsimp_all simp add: propagate_bt_wl_D_heur_def twl_st_heur_def
+            Let_def T' U' rescore_clause_def S' map_fun_rel_def
             list_of_mset2_def vmtf_flush_def RES_RES2_RETURN_RES RES_RETURN_RES uminus_\<A>\<^sub>i\<^sub>n_iff
             get_fresh_index_def RES_RETURN_RES2 RES_RES_RETURN_RES2 lit_of_hd_trail_def
             RES_RES_RETURN_RES lbd_empty_def get_LBD_def DECISION_REASON_def
             all_atms_def[symmetric] All_atms_rew learned_clss_count_def all_atms_st_def
-            aivdom_inv_dec_intro_add_mset
+            aivdom_inv_dec_intro_add_mset valid_arena_update_lbd old clss_size_corr_intro(2)
             intro!: valid_arena_update_lbd aivdom_inv_intro_add_mset
             simp del: isasat_input_bounded_def isasat_input_nempty_def
           dest: valid_arena_one_notin_vdomD
             get_learned_count_learned_clss_countD)
-          (intro conjI,  auto
+          (auto
           intro!: valid_arena_update_lbd aivdom_inv_intro_add_mset
           simp: vdom_m_simps5
             simp del: isasat_input_bounded_def isasat_input_nempty_def
@@ -2395,36 +2431,45 @@ proof -
        \<open>LK' = lit_of (hd (get_trail_wl T'))\<close>
        \<open>LK = LK'\<close>
        using KK' SS' S' by (auto simp: T')
-    obtain vm' W' clvls cach lbd outl stats heur vdom lcount arena D' Q' opts
-      M1'
-      where
-        U: \<open>U = (M1', arena, D', Q', W', vm', clvls, cach, lbd, outl, stats, heur,
-           vdom, lcount, opts, [])\<close> and
+    let ?M1' = \<open>get_trail_wl_heur U\<close>
+    let ?arena = \<open>get_clauses_wl_heur U\<close>
+    let ?D' = \<open>get_conflict_wl_heur U\<close>
+    let ?W' = \<open>get_watched_wl_heur U\<close>
+    let ?vm' = \<open>get_vmtf_heur U\<close>
+    let ?clvls = \<open>get_count_max_lvls_heur U\<close>
+    let ?cach = \<open>get_conflict_cach U\<close>
+    let ?outl = \<open>get_outlearned_heur U\<close>
+    let ?lcount = \<open>get_learned_count U\<close>
+    let ?heur = \<open>get_heur U\<close>
+    let ?lbd = \<open>get_lbd U\<close>
+    let ?aivdom = \<open>isasat_int.get_aivdom U\<close>
+    have
         r': \<open>length (get_clauses_wl_heur U) = r\<close>
             \<open>get_learned_count U = get_learned_count S\<close>
-            \<open>learned_clss_count U \<le> u\<close>
+            \<open>learned_clss_count U \<le> u\<close> and
+      old: \<open>get_old_arena U = []\<close>
       using SS' UU' find_decomp r \<open>(TnC, T') \<in> ?shorter S' S\<close>
         get_learned_count_learned_clss_countD2[of U S]
-      by (cases U) (auto simp: U' T' twl_st_heur_bt_def)
-    let ?vdom = \<open>set (get_vdom_aivdom vdom)\<close>
+      by (auto simp: U' T' twl_st_heur_bt_def)
+    let ?vdom = \<open>set (get_vdom_aivdom ?aivdom)\<close>
     have
-      M'M: \<open>(M1', M1) \<in> trail_pol (all_atms_st U')\<close> and
-      W'W: \<open>(W', W) \<in> \<langle>Id\<rangle>map_fun_rel (D\<^sub>0  (all_atms_st U'))\<close> and
-      vmtf: \<open>vm' \<in> isa_vmtf  (all_atms_st U') M1\<close> and
+      M'M: \<open>(?M1', M1) \<in> trail_pol (all_atms_st U')\<close> and
+      W'W: \<open>(?W', W) \<in> \<langle>Id\<rangle>map_fun_rel (D\<^sub>0  (all_atms_st U'))\<close> and
+      vmtf: \<open>?vm' \<in> isa_vmtf  (all_atms_st U') M1\<close> and
       n_d_M1: \<open>no_dup M1\<close> and
-      empty_cach: \<open>cach_refinement_empty  (all_atms_st U') cach\<close> and
-      \<open>length outl = Suc 0\<close> and
-      outl: \<open>out_learned M1 None outl\<close> and
-      lcount: \<open>clss_size_corr N NE UE NEk UEk NS US N0 U0 lcount\<close> and
+      empty_cach: \<open>cach_refinement_empty  (all_atms_st U') ?cach\<close> and
+      \<open>length ?outl = Suc 0\<close> and
+      outl: \<open>out_learned M1 None ?outl\<close> and
+      lcount: \<open>clss_size_corr N NE UE NEk UEk NS US N0 U0 ?lcount\<close> and
       vdom: \<open>vdom_m (all_atms_st U') W N \<subseteq> ?vdom\<close> and
-      valid: \<open>valid_arena arena N ?vdom\<close> and
-      D': \<open>(D', None) \<in> option_lookup_clause_rel (all_atms_st U')\<close> and
+      valid: \<open>valid_arena ?arena N ?vdom\<close> and
+      D': \<open>(?D', None) \<in> option_lookup_clause_rel (all_atms_st U')\<close> and
       bounded: \<open>isasat_input_bounded (all_atms_st U')\<close> and
       nempty: \<open>isasat_input_nempty (all_atms_st U')\<close> and
-      dist_vdom: \<open>distinct (get_vdom_aivdom vdom)\<close> and
-      aivdom: \<open>aivdom_inv_dec vdom (dom_m N)\<close> and
-      heur: \<open>heuristic_rel (all_atms_st U') heur\<close>
-      using UU' by (auto simp: out_learned_def twl_st_heur_bt_def U U' all_atms_def[symmetric]
+      dist_vdom: \<open>distinct (get_vdom_aivdom ?aivdom)\<close> and
+      aivdom: \<open>aivdom_inv_dec ?aivdom (dom_m N)\<close> and
+      heur: \<open>heuristic_rel (all_atms_st U') ?heur\<close>
+      using UU' by (auto simp: out_learned_def twl_st_heur_bt_def U' all_atms_def[symmetric]
         aivdom_inv_dec_alt_def)
     have [simp]: \<open>C ! 0 = - lit_of (hd M)\<close> and
       n_d: \<open>no_dup M\<close>
@@ -2452,33 +2497,33 @@ proof -
          single_of_mset_def RES_RETURN_RES image_iff)
 
     have [refine0]:
-      \<open>lbd_empty lbd \<le> SPEC (\<lambda>c. (c, ()) \<in> {(c, _). c = replicate (length lbd) False})\<close>
+      \<open>lbd_empty ?lbd \<le> SPEC (\<lambda>c. (c, ()) \<in> {(c, _). c = replicate (length ?lbd) False})\<close>
       by (auto simp: lbd_empty_def)
-    have [refine0]: \<open>mop_isa_length_trail M1' \<le>  \<Down> {(j, _). j = length M1} (RETURN ())\<close>
+    have [refine0]: \<open>mop_isa_length_trail ?M1' \<le>  \<Down> {(j, _). j = length M1} (RETURN ())\<close>
       by (rule order_trans, rule mop_isa_length_trail_length_u[THEN fref_to_Down_Id_keep, OF _ M'M])
         (auto simp: RETURN_def conc_fun_RES)
 
-    have [refine0]: \<open>isa_vmtf_flush_int M1' vm' \<le>
+    have [refine0]: \<open>isa_vmtf_flush_int ?M1' ?vm' \<le>
          SPEC(\<lambda>c. (c, ()) \<in> {(vm', _). vm' \<in> isa_vmtf (all_atms_st U') M1})\<close>
       for vm i L
     proof -
       obtain vm0 where
-        vm: \<open>(vm', vm0) \<in> Id \<times>\<^sub>r distinct_atoms_rel (all_atms_st U')\<close> and
+        vm: \<open>(?vm', vm0) \<in> Id \<times>\<^sub>r distinct_atoms_rel (all_atms_st U')\<close> and
         vm0: \<open>vm0 \<in> vmtf (all_atms_st U') M1\<close>
-        using vmtf unfolding isa_vmtf_def by (cases vm') auto
+        using vmtf unfolding isa_vmtf_def by (cases ?vm') auto
       show ?thesis
         apply (rule order.trans)
-        apply (rule isa_vmtf_flush_int[THEN fref_to_Down_curry, of _ _ M1 vm'])
+        apply (rule isa_vmtf_flush_int[THEN fref_to_Down_curry, of _ _ M1 ?vm'])
         apply ((solves \<open>use M'M in auto\<close>)+)[2]
         apply (subst Down_id_eq)
         apply (rule order.trans)
-        apply (rule vmtf_change_to_remove_order'[THEN fref_to_Down_curry, of \<open>all_atms_st U'\<close> M1 vm0 M1 vm'])
+        apply (rule vmtf_change_to_remove_order'[THEN fref_to_Down_curry, of \<open>all_atms_st U'\<close> M1 vm0 M1 ?vm'])
         subgoal using vm0 bounded nempty by auto
         subgoal using vm by auto
         subgoal by (auto simp: vmtf_flush_def conc_fun_RES RETURN_def intro: isa_vmtfI)
         done
     qed
-    have [refine0]: \<open>get_LBD lbd \<le> SPEC(\<lambda>c. (c, ()) \<in> UNIV)\<close>
+    have [refine0]: \<open>get_LBD ?lbd \<le> SPEC(\<lambda>c. (c, ()) \<in> UNIV)\<close>
       by (auto simp: get_LBD_def)
 
     have tr_S: \<open>(get_trail_wl_heur S, M) \<in> trail_pol (all_atms_st S')\<close>
@@ -2571,15 +2616,24 @@ proof -
       by auto
     have [simp]: \<open>clss_size_corr N NE (add_mset C UE) NEk UEk NS US N0 U0
       (clss_size_incr_lcountUE (get_learned_count S))\<close> for C
-      using lcount UU' r' unfolding U' U
+      using lcount UU' r' unfolding U'
       by (cases S)
        (simp add: twl_st_heur_bt_def clss_size_corr_intro)
 
     show ?thesis
       using empty_cach n_d_M1 W'W outl vmtf C undef uL_M vdom lcount valid D' aivdom
-      unfolding U U' propagate_unit_bt_wl_D_int_def prod.simps hd_SM
+      unfolding U' propagate_unit_bt_wl_D_int_def prod.simps hd_SM
         propagate_unit_bt_wl_alt_def
       apply (rewrite at \<open>let _ = incr_units_since_last_GC (incr_uset _) in _\<close> Let_def)
+      apply (rewrite at  \<open>let _ =  get_trail_wl_heur _ in _ \<close>Let_def)
+      apply (rewrite at  \<open>let _ =  get_clauses_wl_heur _ in _ \<close>Let_def)
+      apply (rewrite at  \<open>let _ =  get_vmtf_heur _ in _ \<close>Let_def)
+      apply (rewrite at  \<open>let _ =  get_lbd _ in _ \<close>Let_def)
+      apply (rewrite at  \<open>let _ =  get_aivdom _ in _ \<close>Let_def)
+      apply (rewrite at  \<open>let _ =  get_watched_wl_heur _ in _ \<close>Let_def)
+      apply (rewrite at  \<open>let _ = get_learned_count _ in _ \<close> Let_def)
+      apply (rewrite at  \<open>let _ = get_heur _ in _ \<close> Let_def)
+      apply (rewrite at  \<open>let _ = get_stats_heur _ in _ \<close> Let_def)
       apply (refine_rcg cons_trail_Propagated_tr2[where \<A> = \<open>all_atms_st U'\<close>])
       subgoal by (auto simp: DECISION_REASON_def)
       subgoal
@@ -2587,7 +2641,7 @@ proof -
            (use undef uL_M in \<open>auto simp: hd_SM all_atms_def[symmetric] T'
 	    lit_of_hd_trail_def S'\<close>)
      subgoal
-       using M'M by (auto simp: U U' lit_of_hd_trail_st_heur_def RETURN_def
+       using M'M by (auto simp: U' lit_of_hd_trail_st_heur_def RETURN_def
            single_of_mset_def vmtf_flush_def twl_st_heur_def lbd_empty_def get_LBD_def
            RES_RES2_RETURN_RES RES_RETURN_RES S' uminus_\<A>\<^sub>i\<^sub>n_iff RES_RES_RETURN_RES
            DECISION_REASON_def hd_SM lit_of_hd_trail_st_heur_def
@@ -2595,7 +2649,7 @@ proof -
            intro!: vmtf_consD
            simp del: isasat_input_bounded_def isasat_input_nempty_def)
      subgoal
-       by (auto simp: U U' lit_of_hd_trail_st_heur_def RETURN_def
+       by (auto simp: U' lit_of_hd_trail_st_heur_def RETURN_def
            single_of_mset_def vmtf_flush_def twl_st_heur_def lbd_empty_def get_LBD_def
            RES_RES2_RETURN_RES RES_RETURN_RES S' uminus_\<A>\<^sub>i\<^sub>n_iff RES_RES_RETURN_RES
            DECISION_REASON_def hd_SM T'
@@ -2604,10 +2658,10 @@ proof -
            simp del: isasat_input_bounded_def isasat_input_nempty_def)
      subgoal
        using bounded nempty dist_vdom r' heur aivdom
-       by (auto simp: U U' lit_of_hd_trail_st_heur_def RETURN_def
+       by (auto simp: U' lit_of_hd_trail_st_heur_def RETURN_def
            single_of_mset_def vmtf_flush_def twl_st_heur_def lbd_empty_def get_LBD_def
          RES_RES2_RETURN_RES RES_RETURN_RES S' uminus_\<A>\<^sub>i\<^sub>n_iff RES_RES_RETURN_RES
-         learned_clss_count_def all_atms_st_def
+         learned_clss_count_def all_atms_st_def old
            DECISION_REASON_def hd_SM All_atms_rew all_atms_def[symmetric]
            intro!: ASSERT_refine_left RES_refine exI[of _ \<open>-lit_of (hd M)\<close>]
            intro!: isa_vmtf_consD2
@@ -2628,7 +2682,9 @@ proof -
         (auto simp:  twl_st_heur_conflict_ana_def trail_pol_def ann_lits_split_reasons_def)
   qed
 
-
+  have H:
+    \<open>(x, y) \<in> twl_st_heur_conflict_ana \<Longrightarrow> fst (get_trail_wl_heur x) \<noteq> [] \<longleftrightarrow> get_trail_wl y \<noteq> []\<close> for x y
+    by (auto simp: twl_st_heur_conflict_ana_def trail_pol_def ann_lits_split_reasons_def)
   have [refine]: \<open>\<And>x y. (x, y)
           \<in> {(S, T).
              (S, T) \<in> twl_st_heur_conflict_ana \<and>
@@ -2637,14 +2693,18 @@ proof -
           \<le> \<Down> {(L, L'). L = L' \<and> L = lit_of (hd (get_trail_wl y))} (mop_lit_hd_trail_wl y)\<close>
     unfolding mop_lit_hd_trail_wl_def lit_of_hd_trail_st_heur_def
     apply refine_rcg
-    subgoal unfolding mop_lit_hd_trail_wl_pre_def mop_lit_hd_trail_l_pre_def mop_lit_hd_trail_pre_def
-     by (auto simp:  twl_st_heur_conflict_ana_def mop_lit_hd_trail_wl_pre_def mop_lit_hd_trail_l_pre_def trail_pol_alt_def
-           mop_lit_hd_trail_pre_def state_wl_l_def twl_st_l_def lit_of_hd_trail_def RETURN_RES_refine_iff)
+    subgoal for x y
+      unfolding mop_lit_hd_trail_wl_pre_def mop_lit_hd_trail_l_pre_def mop_lit_hd_trail_pre_def in_pair_collect_simp
+      by normalize_goal+
+        (simp add: H)
     subgoal for  x y
-      apply simp_all
-      by (subst lit_of_last_trail_pol_lit_of_last_trail[THEN fref_to_Down_unRET_Id, of \<open>get_trail_wl y\<close> \<open>get_trail_wl_heur x\<close> \<open>all_atms_st y\<close>])
-        (auto simp:  twl_st_heur_conflict_ana_def mop_lit_hd_trail_wl_pre_def mop_lit_hd_trail_l_pre_def
+      unfolding mop_lit_hd_trail_wl_pre_def mop_lit_hd_trail_l_pre_def mop_lit_hd_trail_pre_def in_pair_collect_simp
+      apply normalize_goal+
+      apply (subst lit_of_last_trail_pol_lit_of_last_trail[THEN fref_to_Down_unRET_Id, of \<open>get_trail_wl y\<close> \<open>get_trail_wl_heur x\<close> \<open>all_atms_st y\<close>])
+      apply (simp_all add: H)
+      apply (auto simp:  twl_st_heur_conflict_ana_def mop_lit_hd_trail_wl_pre_def mop_lit_hd_trail_l_pre_def
            mop_lit_hd_trail_pre_def state_wl_l_def twl_st_l_def lit_of_hd_trail_def RETURN_RES_refine_iff)
+      done
     done
   have backtrack_wl_alt_def:
     \<open>backtrack_wl S =
@@ -2719,57 +2779,53 @@ lemma le_uint32_max_div_2_le_uint32_max: \<open>a \<le> uint32_max div 2 + 1 \<L
   by (auto simp: uint32_max_def sint64_max_def)
 
 
-lemma propagate_bt_wl_D_heur_alt_def:
-  \<open>propagate_bt_wl_D_heur = (\<lambda>L C (M, N0, D, Q, W0, vm0, y, cach, lbd, outl, stats, heur,
-         vdom, lcount, opts). do {
-      ASSERT(length (get_vdom_aivdom vdom) \<le> length N0);
-      ASSERT(length (get_avdom_aivdom vdom) \<le> length N0);
-      ASSERT(nat_of_lit (C!1) < length W0 \<and> nat_of_lit (-L) < length W0);
-      ASSERT(length C > 1);
-      let L' = C!1;
-      ASSERT(length C \<le> uint32_max div 2 + 1);
-      vm \<leftarrow> isa_vmtf_rescore C M vm0;
-      glue \<leftarrow> get_LBD lbd;
-      let b = False;
-      let b' = (length C = 2);
-      ASSERT(isasat_fast (M, N0, D, Q, W0, vm0, y, cach, lbd, outl, stats, heur,
-         vdom, lcount, opts) \<longrightarrow> append_and_length_fast_code_pre ((b, C), N0));
-      ASSERT(isasat_fast (M, N0, D, Q, W0, vm0, y, cach, lbd, outl, stats, heur,
-         vdom, lcount, opts) \<longrightarrow> clss_size_lcount lcount < sint64_max);
-      (N, i) \<leftarrow> fm_add_new_fast b C N0;
-      ASSERT(update_lbd_pre ((i, glue), N));
-      let N = update_lbd i glue N;
-      ASSERT(isasat_fast (M, N0, D, Q, W0, vm0, y, cach, lbd, outl, stats, heur,
-         vdom, lcount, opts) \<longrightarrow> length_ll W0 (nat_of_lit (-L)) < sint64_max);
-      let W = W0[nat_of_lit (- L) := W0 ! nat_of_lit (- L) @ [(i, L', b')]];
-      ASSERT(isasat_fast (M, N0, D, Q, W0, vm0, y, cach, lbd, outl, stats, heur,
-         vdom, lcount, opts) \<longrightarrow> length_ll W (nat_of_lit L') < sint64_max);
-      let W = W[nat_of_lit L' := W!nat_of_lit L' @ [(i, -L, b')]];
-      lbd \<leftarrow> lbd_empty lbd;
-      j \<leftarrow> mop_isa_length_trail M;
-      ASSERT(i \<noteq> DECISION_REASON);
-      ASSERT(cons_trail_Propagated_tr_pre ((-L, i), M));
-      M \<leftarrow> cons_trail_Propagated_tr (- L) i M;
-      vm \<leftarrow> isa_vmtf_flush_int M vm;
-      heur \<leftarrow> mop_save_phase_heur (atm_of L') (is_neg L') heur;
-      RETURN (M, N, D, j, W, vm, 0,
-        cach, lbd, outl, add_lbd (of_nat glue) stats, heuristic_reluctant_tick (update_propagation_heuristics glue heur),
-        add_learned_clause_aivdom i vdom,
-          clss_size_incr_lcount lcount, opts)
-    })\<close>
-  unfolding propagate_bt_wl_D_heur_def Let_def by (auto intro!: ext)
+(* lemma propagate_bt_wl_D_heur_alt_def:
+ *   \<open>propagate_bt_wl_D_heur = (\<lambda>L C (M, N0, D, Q, W0, vm0, y, cach, lbd, outl, stats, heur,
+ *          vdom, lcount, opts). do {
+ *       ASSERT(length (get_vdom_aivdom vdom) \<le> length N0);
+ *       ASSERT(length (get_avdom_aivdom vdom) \<le> length N0);
+ *       ASSERT(nat_of_lit (C!1) < length W0 \<and> nat_of_lit (-L) < length W0);
+ *       ASSERT(length C > 1);
+ *       let L' = C!1;
+ *       ASSERT(length C \<le> uint32_max div 2 + 1);
+ *       vm \<leftarrow> isa_vmtf_rescore C M vm0;
+ *       glue \<leftarrow> get_LBD lbd;
+ *       let b = False;
+ *       let b' = (length C = 2);
+ *       ASSERT(isasat_fast (M, N0, D, Q, W0, vm0, y, cach, lbd, outl, stats, heur,
+ *          vdom, lcount, opts) \<longrightarrow> append_and_length_fast_code_pre ((b, C), N0));
+ *       ASSERT(isasat_fast (M, N0, D, Q, W0, vm0, y, cach, lbd, outl, stats, heur,
+ *          vdom, lcount, opts) \<longrightarrow> clss_size_lcount lcount < sint64_max);
+ *       (N, i) \<leftarrow> fm_add_new_fast b C N0;
+ *       ASSERT(update_lbd_pre ((i, glue), N));
+ *       let N = update_lbd i glue N;
+ *       ASSERT(isasat_fast (M, N0, D, Q, W0, vm0, y, cach, lbd, outl, stats, heur,
+ *          vdom, lcount, opts) \<longrightarrow> length_ll W0 (nat_of_lit (-L)) < sint64_max);
+ *       let W = W0[nat_of_lit (- L) := W0 ! nat_of_lit (- L) @ [(i, L', b')]];
+ *       ASSERT(isasat_fast (M, N0, D, Q, W0, vm0, y, cach, lbd, outl, stats, heur,
+ *          vdom, lcount, opts) \<longrightarrow> length_ll W (nat_of_lit L') < sint64_max);
+ *       let W = W[nat_of_lit L' := W!nat_of_lit L' @ [(i, -L, b')]];
+ *       lbd \<leftarrow> lbd_empty lbd;
+ *       j \<leftarrow> mop_isa_length_trail M;
+ *       ASSERT(i \<noteq> DECISION_REASON);
+ *       ASSERT(cons_trail_Propagated_tr_pre ((-L, i), M));
+ *       M \<leftarrow> cons_trail_Propagated_tr (- L) i M;
+ *       vm \<leftarrow> isa_vmtf_flush_int M vm;
+ *       heur \<leftarrow> mop_save_phase_heur (atm_of L') (is_neg L') heur;
+ *       RETURN (M, N, D, j, W, vm, 0,
+ *         cach, lbd, outl, add_lbd (of_nat glue) stats, heuristic_reluctant_tick (update_propagation_heuristics glue heur),
+ *         add_learned_clause_aivdom i vdom,
+ *           clss_size_incr_lcount lcount, opts)
+ *     })\<close>
+ *   unfolding propagate_bt_wl_D_heur_def Let_def by (auto intro!: ext) *)
 
 
 lemma propagate_bt_wl_D_fast_code_isasat_fastI2: \<open>isasat_fast b \<Longrightarrow>
-       b = (a1', a2') \<Longrightarrow>
-       a2' = (a1'a, a2'a) \<Longrightarrow>
-       a < length a1'a \<Longrightarrow> a \<le> sint64_max\<close>
+       a < length (get_clauses_wl_heur b) \<Longrightarrow> a \<le> sint64_max\<close>
   by (cases b) (auto simp: isasat_fast_def)
 
 lemma propagate_bt_wl_D_fast_code_isasat_fastI3: \<open>isasat_fast b \<Longrightarrow>
-       b = (a1', a2') \<Longrightarrow>
-       a2' = (a1'a, a2'a) \<Longrightarrow>
-       a \<le> length a1'a \<Longrightarrow> a < sint64_max\<close>
+       a \<le> length (get_clauses_wl_heur b) \<Longrightarrow> a < sint64_max\<close>
   by (cases b) (auto simp: isasat_fast_def sint64_max_def uint32_max_def)
 
 end
